code/experimental/rsapss/Hacl.Spec.Bignum.Multiplication.fst
@@ -1,0 +1,65 @@
+module Hacl.Spec.Bignum.Multiplication
+
+open FStar.Mul
+
+open Lib.IntTypes
+open Lib.Sequence
+open Lib.LoopCombinators
+
+open Hacl.Spec.Bignum
+open Hacl.Spec.Bignum.Base
+open Hacl.Spec.Bignum.Addition
+
+
+#reset-options "--z3rlimit 50 --max_fuel 0 --max_ifuel 0"
+
+val bn_mul_by_limb_addj_f:
+    #aLen:size_nat
+  -> a:lbignum aLen
+  -> l:uint64
+  -> res:lbignum aLen
+  -> i:size_nat{i < aLen}
+  -> c:uint64 ->
+  uint64 & uint64 // carry & out
+
+let bn_mul_by_limb_addj_f #aLen a l res i c =
+  mul_carry_add_u64 a.[i] l c res.[i]
+
+
+val bn_mul_by_limb_addj:
+    #aLen:size_nat
+  -> a:lbignum aLen
+  -> l:uint64
+  -> res:lbignum aLen ->
+  uint64 & lbignum aLen
+
+let bn_mul_by_limb_addj #aLen a l res =
+  generate_elems aLen aLen (bn_mul_by_limb_addj_f a l res) (u64 0)
+
+
+val bn_mul_:
+    #aLen:size_nat
+  -> #bLen:size_nat{aLen + bLen <= max_size_t}
+  -> a:lbignum aLen
+  -> b:lbignum bLen
+  -> j:size_nat{j < bLen}
+  -> res:lbignum (aLen + bLen) ->
+  lbignum (aLen + bLen)
+
+let bn_mul_ #aLen #bLen a b j res =
+  let res' = sub res j aLen in
+  let c, res' = bn_mul_by_limb_addj #aLen a b.[j] res' in
+  let res = update_sub res j aLen res' in
+  res.[aLen + j] <- c
+
+
+val bn_mul:
+    #aLen:size_nat
+  -> #bLen:size_nat{aLen + bLen <= max_size_t}
+  -> a:lbignum aLen
+  -> b:lbignum bLen ->
+  lbignum (aLen + bLen)
+
+let bn_mul #aLen #bLen a b =
+  let res = create (aLen + bLen) (u64 0) in
+  repeati bLen (bn_mul_ #aLen #bLen a b) res
